refactor trace execution semantics to integrate trace into state

src/Facade.v
@@ -26,8 +26,6 @@ Ltac apply_in_hyp lem :=
   | [ H : _ |- _ ] => eapply lem in H
   end.
 
-Local Open Scope string_scope.
-
 Definition addr := nat.
 Definition valu := nat.
 
@@ -71,79 +69,109 @@ Hint Constructors exec.
 
 Definition trace := list (addr * valu).
 
-Inductive step_trace T : diskstate -> prog T -> diskstate -> prog T -> trace -> Prop :=
-| StepTRead : forall d a rx, step_trace d (Read a rx) d (rx (d a)) []
-| StepTWrite : forall d a v rx, step_trace d (Write a v rx) (upd a v d) (rx tt) [(a, v)].
+Inductive step_trace T : diskstate -> trace -> prog T -> diskstate -> trace -> prog T -> Prop :=
+| StepTRead : forall d tr a rx , step_trace d tr (Read a rx) d tr (rx (d a))
+| StepTWrite : forall d tr a v rx, step_trace d tr (Write a v rx) (upd a v d) ((a, v) :: tr) (rx tt).
 
 Hint Constructors step_trace.
 
-Inductive exec_trace T : diskstate -> prog T -> outcome T -> trace -> Prop :=
-| XTStep : forall d p d' p' out t1 t2 t,
-  t = (t1 ++ t2)%list -> (* TODO: which order? *)
-  step_trace d p d' p' t1 ->
-  exec_trace d' p' out t2 ->
-  exec_trace d p out t
-| XTFail : forall d p, (~exists d' p', step d p d' p') ->
+Inductive exec_trace T : diskstate -> trace -> prog T -> outcome T -> trace -> Prop :=
+| XTStep : forall d p d' p' out tr tr' tr'',
+  step_trace d tr p d' tr' p' ->
+  exec_trace d' tr' p' out tr'' ->
+  exec_trace d tr p out tr''
+| XTFail : forall d p tr, (~exists d' p', step d p d' p') ->
   (~exists r, p = Done r) ->
-  exec_trace d p (Failed T) []
-| XTCrash : forall d p, exec_trace d p (Crashed T d) []
-| XTDone : forall d v,
-  exec_trace d (Done v) (Finished d v) [].
+  exec_trace d tr p (Failed T) tr
+| XTCrash : forall d p tr, exec_trace d tr p (Crashed T d) tr
+| XTDone : forall d v tr,
+  exec_trace d tr (Done v) (Finished d v) tr.
 
 Hint Constructors exec_trace.
 
-Definition computes_to_trace A (p : forall T, (A -> prog T) -> prog T) (d d' : diskstate) (tr : trace) (x : A) :=
-  forall T (rx : A -> prog T) d'' tr' (y : T),
-    exec_trace d' (rx x) (Finished d'' y) tr' <-> exec_trace d (p T rx) (Finished d'' y) (tr ++ tr')%list.
+Definition computes_to_trace A (p : forall T, (A -> prog T) -> prog T) (d d' : diskstate) (tr tr' : trace) (x : A) :=
+  forall T (rx : A -> prog T) d'' tr'' (y : T),
+    exec_trace d' tr' (rx x) (Finished d'' y) tr'' <-> exec_trace d tr (p T rx) (Finished d'' y) tr''.
 
 Definition computes_to A (p : forall T, (A -> prog T) -> prog T) (d d' : diskstate) (x : A) :=
   forall T (rx : A -> prog T) d'' (y : T),
     exec d' (rx x) (Finished d'' y) <-> exec d (p T rx) (Finished d'' y).
 
-Lemma step_trace_equiv : forall T d p d' p',
-  @step T d p d' p' <-> exists tr, step_trace d p d' p' tr.
+Lemma step_trace_equiv_1 : forall T d p d' p',
+  @step T d p d' p' -> forall tr, exists tr', step_trace d tr p d' (tr' ++ tr) p'.
 Proof.
   intros.
-  split; intro.
-  + destruct H; eauto.
-  + destruct H. destruct H; eauto.
+  destruct H; eexists; try solve [instantiate (1 := []); eauto]; try solve [instantiate (1 := [_]); simpl; eauto].
 Qed.
 
-Lemma exec_trace_equiv : forall T d p out,
-  @exec T d p out <-> exists tr, exec_trace d p out tr.
+Lemma step_trace_equiv_2 : forall T d p d' p',
+  (exists tr tr', step_trace d tr p d' (tr' ++ tr) p') -> @step T d p d' p'.
 Proof.
   intros.
-  split; intro.
-  + induction H; eauto.
-    apply_in_hyp step_trace_equiv.
-    repeat deex. eauto.
-  + deex.
-    induction H; eauto.
-    econstructor; eauto.
-    eapply step_trace_equiv; eauto.
+  repeat deex. destruct H; eauto.
 Qed.
 
-Lemma computes_to_trace_prefix : forall A p d d' tr x,
-  @computes_to_trace A p d d' tr x ->
-  forall T rx d'' y tr0,
-  exec_trace d (p T rx) (Finished d'' y) tr0 ->
-  exists tr', tr0 = (tr ++ tr')%list.
-Proof.
-  intros.
-  unfold computes_to in *.
-  (* I suspect this is true but unprovable, because it relies on "Theorems for Free"-style parametricity. *)
-Abort.
+Hint Resolve step_trace_equiv_2.
 
-Lemma computes_to_equiv : forall A p d d' x,
-  @computes_to A p d d' x <-> exists tr, computes_to_trace p d d' tr x.
+Lemma step_trace_prepends : forall T d tr p d' tr' p',
+  @step_trace T d tr p d' tr' p' -> exists tr0, tr' = tr0 ++ tr.
 Proof.
-  split; intro.
-  admit.
   intros.
-  unfold computes_to.
-  deex; eapply exec_trace_equiv; apply_in_hyp exec_trace_equiv; deex.
-  eexists. eapply H. eauto.
-Abort.
+  destruct H; eexists.
+  + instantiate (1 := []); reflexivity.
+  + instantiate (1 := [_]); reflexivity.
+Qed.
+
+Lemma exec_trace_prepends : forall T d tr p tr' out,
+  @exec_trace T d tr p out tr' -> exists tr0, tr' = tr0 ++ tr.
+Proof.
+  intros.
+  induction H; try solve [ exists []; trivial ].
+  apply_in_hyp step_trace_prepends. repeat deex. eexists. apply app_assoc.
+Qed.
+
+
+Lemma step_trace_append : forall T d tr p d' tr' p' tr0,
+  @step_trace T d tr p d' tr' p' -> step_trace d (tr ++ tr0) p d' (tr' ++ tr0) p'.
+Proof.
+  intros.
+  destruct H; eauto.
+  econstructor.
+Qed.
+
+Hint Resolve step_trace_append.
+
+Lemma exec_trace_append : forall T d tr p tr' out tr0,
+  @exec_trace T d tr p out tr' -> exec_trace d (tr ++ tr0) p out (tr' ++ tr0).
+Proof.
+  intros.
+  induction H; eauto.
+  econstructor. eapply step_trace_append; eauto. eauto.
+Qed.
+
+Hint Resolve exec_trace_append.
+
+Lemma exec_trace_equiv_1 : forall T d p out,
+  @exec T d p out -> forall tr, exists tr', exec_trace d tr p out (tr' ++ tr).
+Proof.
+  intros. revert tr.
+  induction H; try solve [ exists []; eauto].
+  intro.
+  apply_in_hyp step_trace_equiv_1.
+  deex. specialize (IHexec tr'). deex. eauto.
+Qed.
+
+Lemma exec_trace_equiv_2 : forall T d p out,
+  (exists tr tr', exec_trace d tr p out (tr' ++ tr)) -> @exec T d p out.
+Proof.
+  intros.
+  repeat deex.
+  induction H; eauto.
+  econstructor; eauto.
+  assert (H2 := H).
+  apply_in_hyp step_trace_prepends.
+  repeat deex. eauto.
+Qed.
 
 Definition label := string.
 Definition var := string.
@@ -450,6 +478,8 @@ Proof.
 Qed.
 
 Hint Resolve ret_computes_to_refl.
+
+Local Open Scope string_scope.
 
 
 Example micro_noop : sigT (fun p => forall d0,
